<section xml:id="sec-examples-subrings-ideals">
	<title>Examples of subrings and ideals</title>
	<introduction>
		We give several examples of subrings and ideals.
	</introduction>
	<example xml:id="def-centralizer">
		<title>(Centralizer)</title>
		<statement>
			Let <m>R</m> be a ring and <m>S</m> be a nonempty subset of <m>R</m>. The <term>centralizer of <m>S</m> in <m>R</m></term> is the set of all those elements of <m>R</m> that commutes with every element of <m>S</m>. It is denoted by <m>C_R(S)</m>. Thus,
			<me>C_R(S)=\{r\in R:rs=sr\;\text{for all}\;s\in S\}.</me>
			Verify that <m>C_R(S)</m> is a subring of <m>R</m>.
		</statement>
	</example>
	<example xml:id="def-center">
		<title>(Center of a ring)</title>
		<statement>
			The center of a ring <m>R</m>, <m>\mathcal{Z}(R)</m> is the centralizer of <m>R</m> in <m>R</m>. Thus,
			<me>\mathcal{Z}(R)=\{r\in R:rx=xr\;\text{for all}\;x\in R\}.</me>
			The center of <m>R</m> is a subring of <m>R</m>.
		</statement>
	</example>
	<example xml:id="subrings-of-matrices">
		<title>(Certain subrings of a matrix ring)</title>
		Let <m>M_n(R)</m> be the ring of <m>n\times n</m> matrices over a ring <m>R</m>. Following subsets of <m>M_n(R)</m> are subrings.
		<ol>
			<li>Upper triangular matrices: <m>U_n(R)=\{(a_{ij})\in M_n(R):a_{ij}=0\text{ for }i\gt j\}</m></li>
			<li>Lower triangular matrices: <m>L_n(R)=\{(a_{ij})\in M_n(R):a_{ij}=\text{ for }i\lt j\}</m></li>
			<li>Diagonal matrices: <m>D_n=\{(a_{ij})\in M_n(R):a_{ij}=0\text{ for all }i\neq j\}</m></li>
		</ol>
	</example>
	<example xml:id="idealizer">
		<title>(Idealizer)</title>
		<statement>
			Let <m>I</m> be a right ideal of a ring <m>R</m>. The <term>idealizer of <m>I</m></term> is 
			<me>S=\{r\in R:rI\subset I\}.</me>
			Note that the idealizer of <m>I</m> is a subring containing <m>I</m> as a two-sided ideal.
		</statement>
	</example>
	<example xml:id="ideal-generated-by-finite-set">
		<title>(Ideal generated by a finite set)</title>
		<statement>
			<p>
				Let <m>R</m> be a ring and let <m>r_1,r_2,\ldots,r_n\in R</m>. The <term>ideal generated by <m>r_1,\ldots,r_n</m></term> is 
				<me>(r_1,\ldots,r_n)=\left\{\sum_{i=1}^n\sum_{j=1}^{m_i}x_{ij}r_iy_{ij}:x_{ij},y_{ij}\in R\;\text{and}\;n,m_i\in\N\right\}.</me>
			</p>
			<p>
				A particular case is the <term>principal ideal generated by <m>r</m></term>:
			<me>(r)=RrR=\left\{\sum_{i=1}^nx_iry_i:n\in\mathbb{N}\;\text{and}\;x_i,y_i\in R\right\}.</me>
		</p>
		</statement>
	</example>
	<example xml:id="ideals-of-Z">
	    <title>(Ideals of <m>\Z</m>)</title>
	    <statement>
	    	Note that <m>\Z</m> is an integral domain. Hence, every left ideal of <m>\Z</m> is also a right ideal of <m>\Z</m>. In other words, every ideal of <m>\Z</m> is a two-sided ideal. Let <m>I</m> be a nonzero ideal of <m>\Z</m>. Suppose that <m>n\in I</m> is the least positive integer in <m>I</m>. We claim that <m>n</m> generates <m>I</m>, i.e., <m>(n)=I</m>. Since <m>n\in I</m> we have, using same actions defined in <xref ref="left-action"/> and <xref ref="right-action"/>, <m>\underbrace{n+n+\cdots+n}_{m\text{-times}}=mn\in I</m> for any <m>m\in\Z</m>. Hence <m>(n)\subseteq I</m>. Suppose that <m>s\in I</m>. The division algorithm gives the following.
	    	<me>s=nq+r\quad\text{where}\;0\leq r\lt n</me>
	    	Suppose that <m>r\neq 0</m>. Since <m>s</m> and <m>nq\in I</m> we get <m>r=s-nq\in I</m>. This is a contradiction because <m>n</m> is the least positive integer in <m>I</m>. Therefore, we must have <m>r=0</m>, i.e., <m>s=nq\in (n)</m>. We thus get <m>I=(n)</m>.
	    </statement>
	</example>
	<example xml:id="ideals-of-division-rings">
		<title>(Ideals of division rings)</title>
		<statement>
			Let <m>I</m> be a nonzero left ideal of a division ring <m>D</m>. Let <m>d\in I</m> be a nonzero element. Hence there exists <m>e\in D</m> such that <m>1=de=ed</m>. In particular, <m>1=ed\in I</m> and hence for any <m>x\in D</m> we have <m>x=x1\in I</m>. This shows that every nonzero left ideal of <m>D</m> is <m>D</m>. Similarly, every nonzero right ideal of a division ring will be the whole ring.
		</statement>
	</example>
	<example xml:id="left-right-ideals-of-endomorphism-ring">
		<title>(Left ideals and right ideals of Endomorphism ring of a vector space)</title>
		<statement>
			<p>
				Let <m>V</m> be a finite-dimensional vector space over a field <m>F</m> and let <m>U</m> be a subspace of <m>V</m>. We consider an <m>F</m>-linear map <m>T\colon V\to U</m>, by composing it with the inclusion <m>i\colon U\to V</m>, to be an <m>F</m>-endomorphism. In this way, we consider <m>\Hom_F(V,U)</m> as a subset of <m>\End_F(V)</m>. Moreover, <m>\Hom_F(V,U)</m> is a subgroup of <m>\End_F(V)</m>. Let <m>f\in\End_F(V)</m> and <m>T\in\Hom_F(V,U)</m>. Thus,
			<me>V\xrightarrow{f}V\xrightarrow{T}U</me>
			shows that <m>T\circ f\in\Hom_F(V,U)</m>. Therefore, <m>\Hom_F(V,U)</m> is a right ideal of <m>\End_F(V)</m>. In fact, there is a one-one correspondence between subspaces <m>U</m> of <m>V</m> and right ideals of <m>\End_F(V)</m> given by <m>U\mapsto\Hom_F(V,U)</m>.
		</p>
		<p>
		Indeed, suppose that <m>I</m> is a right ideal of <m>\End_F(V)</m>. Consider the following subspace.
	<me>U=\langle{\rm Im}(f):f\in I\rangle</me>
	Thus <m>I\subseteq\Hom_F(V,U)</m>. Let <m>\{u_1,\ldots,u_r\}</m> be a basis for <m>U</m> and suppose that <m>w_i\in V</m> are such that <m>f_i(w_i)=u_i</m> for some <m>f_i\in I</m><fn>That is, we are assuming that <m>\{u_i\}\subset\bigcup_{f\in I}{\rm Im}(f)</m>. Indeed, we may consider <m>\{u_i\}</m> to be the maximal linearly independent subset of <m>\bigcup_{f\in I}{\rm Im}(f)</m>.</fn>
	<!--\footnote{That is, we are assuming that $\{u_i\}\subset\bigcup_{f\in I}{\rm Im}(f)$. Indeed, we may consider $\{u_i\}$ to be the maximal linearly independent subset of $\bigcup_{f\in I}{\rm Im}(f)$.}.-->
	 Note that we may have <m>f_i=f_j</m> for <m>i\neq j</m>. Let <m>\{v_1,\ldots,v_n\}</m> be a basis of <m>V</m> and let <m>f\in\Hom_F(V,U)</m>. Assume that an <m>F</m>-linear map <m>f</m> is given as follows. 
	<me>f(v_k)=\sum_{\ell=1}^{r}a_{\ell k}u_\ell</me>
	We consider, for each <m>\ell\in\{1,2,\ldots,r\}</m>, <m>E_\ell\in\Hom_F(V,U)</m> as follows:
	<me>E_\ell(v_k)=a_{\ell k}w_{\ell},\text{ where }k\in\{1,2,\ldots,n\}</me>
	Hence for every <m>\ell\in\{1,2,\ldots,r\}</m> we get
	<me>f_{\ell}\circ E_\ell(v_k)=a_{\ell k}u_\ell</me>
	Since <m>f_\ell</m> belongs to a right ideal <m>I</m>, we must have <m>f_\ell\circ E_\ell\in I</m>.
	Therefore,
	<md><mrow>
		f(v_k)\amp=\sum_{\ell=1}^{r}a_{\ell k}u_\ell</mrow><mrow>\amp=\sum_{\ell=1}^{r}f_\ell\circ E_\ell(v_k)\in I</mrow></md>
We thus get <m>\Hom_F(V,U)\subseteq I</m>.
		</p>
		<p>
			Similarly, there is a one-one correspondence between subspaces <m>U</m> of <m>V</m> and left ideals of <m>\End_F(V)</m> given by <m>U\mapsto\Hom_F(V/U,V)</m>.
		</p>
		</statement>
	</example>
	<example xml:id="ideals-of-rings-and-matrix-rings">
		<title>(Correspondence between ideals of a ring <m>R</m> and ideals of a matrix ring over <m>R</m>)</title>
		<statement>
			Let <m>R</m> be a ring and let <m>M_n(R)</m> be the ring of matrices over <m>R</m>. If <m>S</m> is a subset of <m>R</m> we denote by <m>M_n(S)</m> the set of all <m>n\times n</m> matrices with entries from <m>S</m>.
			<p>
				We show that every ideal, i.e., every two-sided ideal of <m>M_n(R)</m> is of the form <m>M_n(I)</m> for some ideal <m>I</m> of <m>R</m>.
			</p>
			<p>
				We leave it to the reader to verify that if <m>I</m> is an ideal of <m>R</m> then <m>M_n(I)</m> is an ideal of <m>M_n(R)</m>. 
			</p>
			<p>
				Suppose that <m>\mathcal{J}</m> be an ideal of <m>M_n(R)</m>. Consider the following subset of <m>R</m>.
				<me>I=\{a\in R:a\text{ is the }(1,1)\text{-th entry of }A\in\mathcal{J}\}</me>
				The set <m>I</m> is an ideal of <m>R</m>. Let <m>E_{ij}</m> be a matrix such that <m>(i,j)</m>-th entry is <m>1</m> and all other entries are zero. Then for any <m>A\in M_n(R)</m> we have the following.
				<me>E_{ij}AE_{k\ell}=a_{jk}E_{i\ell}</me> Therefore, for <m>A\in\mathcal{J}</m> we have
				<me>E_{1j}AE_{k1}=a_{jk}E_{11}\in\mathcal{J}.</me>
				By the construction of <m>I</m> we get that <m>a_{jk}\in I</m> for any <m>j,k\in\{1,2,\ldots,n\}</m>. In particular, <m>\mathcal{J}\subseteq M_n(I)</m>.
			</p>
			<p>
				Conversely, suppose <m>B=(b_{ij})\in M_n(I)</m>. By the construction of <m>I</m>, <m>b_{ij}</m> is the <m>(1,1)</m>-th entry of some <m>B^\prime\in\mathcal{J}</m> (here <m>B^\prime</m> may depend on <m>b_{ij}</m>). Thus, <m>E_{i1}B^\prime E_{1j}=b_{ij}E_{ij}\in\mathcal{J}</m>. Hence, <m>\sum b_{ij}E_{ij}=B^\prime\in\mathcal{J}</m> and therefore, <m>M_{n}(I)\subseteq\mathcal{J}</m>.
			</p>
		</statement>
	</example>
	<example xml:id="annihilator-of-ideal">
		<title>(Annihilators)</title>
		<statement>
			Let <m>R</m> be a ring and <m>I</m> be a right ideal of <m>R</m>. The <term>annihilator</term> of <m>I</m> is defined as follows.
			<me>I^0=\{r\in R:rx=0\;\text{for all}\;x\in I\}</me>
			The annihilator of a right ideal is a left ideal of <m>R</m>.
			<p>Similarly, if <m>J</m> is a left ideal of <m>R</m> we define the annihilator of <m>J</m> as follows.
			<me>J^0=\{r\in R:xr=0\;\text{for all}\;x\in J\}</me>
		The annihilator <m>J^0</m> is a right ideal of <m>R</m>.
		</p>
		</statement>
	</example>
	<example xml:id="kernel-of-evaluation-map">
		<title>(Kernel of the evaluation map)</title>
		<statement>
			Let <m>F</m> be a field and let <m>F[X]</m> be the ring of polynomials over <m>F</m> in one variable. Fix <m>\alpha\in F</m>. We define the <term>evaluation map</term> at <m>\alpha\in F</m> as follows.
			<me>\ev_{\alpha}\colon F[X]\to F\quad\text{given by}\quad\sum_{i=1}^na_iX^i\mapsto\sum_{i=1}^na_i\alpha^i</me>
			Verify that the following set is an ideal of <m>F[X]</m>:
			<me>\{f\in F[X]:\ev_{\alpha}(f)=0\}</me>
		</statement>
	</example>
	<example xml:id="maximal-ideals-of-polynomial-ring">
		<title>(Some ideals in polynomial ring in several variables)</title>
		<statement>
			Let <m>\C[X_1,X_2,\ldots,X_n]</m> be the polynomial ring in <m>n</m> variables. Fix <m>a_1,a_2,\ldots,a_n\in\C</m>. The following set is a two-sided ideal of <m>\C[X_1,X_2,\ldots,X_n]</m>.
			<me>\mathfrak{m}=(X_1-a_1,X_2-a_2,\ldots,X_n-a_n)</me>
		</statement>
	</example>
	<example xml:id="continuous-functions-vanishing-at-point">
		<title>(Continuous functions vanishing at a point)</title>
		Let <m>C(I)</m> be the ring of continuous real-valued functions on a nonempty interval <m>I\subseteq\R</m> (see <xref ref="ring-of-continuous-real-valued-functions"/>). Fix <m>a_0\in I</m>. Consider the set of all continuous functions on <m>I</m> vanishing at <m>a_0</m> i.e.,
		<me>\mathfrak{m}=\{f\in C(I):f(a_0)=0\}.</me>
		If <m>f,g\in\mathfrak{m}</m> then <m>f-g\in\mathfrak{m}</m>. For any <m>g,h\in C(I)</m> and <m>f\in\mathfrak{m}</m> we have <m>(f\cdot g)(a_0)=f(a_0)g(a_0)=0</m> and <m>(h\cdot f)(a_0)=h(a_0)f(a_0)=0</m>. Thus, <m>\mathfrak{m}</m> is a two-sided ideal of <m>C(I)</m>.
	</example>
	<example xml:id="ideals-in-product-ring">
	<title>(Ideals in product ring)</title>
	<statement>
		Let <m>R</m> and <m>S</m> be two rings and consider the product ring <m>R\times S</m>. If <m>I\subseteq R</m> and <m>J\subseteq S</m> are ideals then <m>I\times J</m> is an ideal of <m>R\times S</m>.
	</statement>
</example>
</section>